Verse/PrettyPrint.v
@@ -2,7 +2,6 @@ Require Import String.
 Require Import Strings.Ascii.
 Require Import List.
 Require Import NPeano.
-Require Verse.Word.
 Import ListNotations.
 
 (* Wadler Pretty printer *)
@@ -118,11 +117,9 @@ Module Internal.
 End Internal.
 
 Definition decimal n := text (Internal.nat_to_str n).
-Definition hexadecimal {n : nat} (u : Word.t (4 * n)) := text (Word.hex u).
-
 
 Class PrettyPrint a := { doc : a -> Doc}.
 
 Instance string_pretty : PrettyPrint string := { doc := text }.
 Instance nat_pretty    : PrettyPrint nat    := { doc := decimal }.
-Instance word_pretty {n : nat} : PrettyPrint (Word.t (4 * n)) := { doc := @hexadecimal n  }.
+
